\documentclass[10pt]{article}

\usepackage{amsmath,amssymb,bm}
\usepackage[a4paper]{geometry}

%\newcommand{\Like}[1]{\mathcal{L} \left( #1 \right)}
%\newcommand{\var}[1]{\mathrm{var} \left( #1 \right)}
%\newcommand{\E}[2][]{\mathbb{E}_{#1} \left[ #2 \right]}
%\newcommand{\Log}[1]{\log \left( #1 \right)}
%\newcommand{\KL}[2]{\mathrm{KL} \left( #1 \vert\vert #2 \right)}
\newcommand{\Angle}[1]{\left \langle #1 \right \rangle}
\newcommand{\Eq}[1]{\Angle{#1}_Q}
\newcommand{\N}[2][]{\mathcal{N} \left( #1,#2 \right)}
\newcommand{\Det}[1]{\left| #1 \right|}
\newcommand{\Tr}[1]{Tr\left( #1 \right)}

\begin{document}

	\begin{align}
		\mathcal{L}(q)&=\int Q(\theta) \ln{\frac{p(t,\theta)}{Q(\theta)}} \, d\theta \\
		&=\Eq{\ln{\frac{p(t,\theta)}{Q(\theta)}}} \\
		&=\underbrace{\Eq{\ln{p(t,\theta)}}}_{(1)} - \underbrace{\Eq{\ln{q(\theta)}}}_{(2)}
	\end{align}
	
	\begin{align}
		\Eq{\ln{p(\bm{t},\theta)}}=&\Eq{\ln{p(\bm{t},\bm{X},\bm{m},\bm{W},z,\sigma^{-2})}} \\
		=&\Eq{\ln{p(\bm{t}|\bm{X},\bm{m},\bm{W},z,\sigma^{-2})p(\bm{X})p(\bm{m})p(\bm{W} \vert z)p(z)p(\sigma^{-2})}} \\
		=&\underbrace{\Eq{\ln{p(\bm{t}|\bm{X},\bm{m},\bm{W},\sigma^{-2},z)}}}_{(3)}+\underbrace{\Eq{\ln{p(\bm{X})}}}_{(4)}+\underbrace{\Eq{\ln{p(\bm{m})}}}_{(5)}+\\
		& \underbrace{\Eq{\ln{p(\bm{W}\vert z)}}}_{(6)}+\underbrace{\Eq{\ln{p(z)}}}_{(8)}+\underbrace{\Eq{\ln{p(\sigma^{-2})}}}_{(7)} \nonumber
	\end{align}
	
	\begin{align}
		\Eq{\ln{p(\bm{t}|\bm{\theta)}}}=&\Eq{\ln{\prod_{n=1}^{N}{p(t_n|\bm{X},\bm{m},\bm{W},\sigma^{-2},z)}}} \\
		=&\Eq{\ln{\prod_{n=1}^{N}{\N[t_n \mid \bm{W}z+\bm{m}]{\sigma^2\bm{I}}}}} \\
		=&\Eq{\sum_{n=1}^{N}{\ln{\N[t_n \mid \bm{W}z+\bm{m}]{\sigma^2\bm{I}}}}} \\
		=&-\frac{Nd}{2}\ln{2\pi}+\frac{dN}{2}\Eq{\ln{\sigma^{-2}}}-\Eq{\sigma^{-2}}\left(\frac{1}{2}\sum_{n=1}^{N}{\gamma_n} \right) \\
		=&\frac{dN}{2}(\psi(\tilde{c}_{\sigma^{-2}})-\ln(\tilde{d}_{\sigma^{-2}}))-\Eq{\sigma^{-2}}\left(\tilde{d}_{\sigma^{-2}}-b\right) + const \\
		=&-\frac{dN}{2}\ln(\tilde{d}_{\sigma^{-2}})-\Eq{\sigma^{-2}}\left(\tilde{d}_{\sigma^{-2}}-b\right) + const
	\end{align}
	\begin{align}
		\frac{1}{2}\sum_{n=1}^N \gamma_n=&\frac{1}{2}\sum_{n=1}^N\langle(t_n-\bm{W}x_n-\bm{m})^T(t_n-\bm{W}x_n-\bm{m})\rangle_Q \\
		=& \frac{1}{2}\sum_{n=1}^N \langle \|t_n\|^2+\|\bm{m}\|^2+x_n^TW^TWx_n \\
		&-2t_n^T\bm{W}x_n-2t_n^T\bm{m}+2\bm{m}^T\bm{W}x_n \rangle_Q \nonumber \\ 
		=&\frac{1}{2}\sum_{n=1}^N\|t_n\|^2+\Angle{\|\bm{m}\|^2}+\Tr{\Angle{W^TW}\Angle{x_nx_n^T}} \\
		&-2t_n^T\Angle{\bm{W}}\Angle{x_n}-2t_n^T\Angle{\bm{m}}+2\Angle{\bm{m}^T}\Angle{\bm{W}}\Angle{x_n} \\
		=& \tilde{d}_{\sigma^{-2}}-b
	\end{align}
	
	\begin{align}
		\Eq{\ln{p(\bm{X})}}=&\Eq{\ln{\prod_{n=1}^{N}{N(x_n|\bm{0},\bm{I}_q)}}} \\
		=&\Eq{\sum_{n=1}^{N}{\ln{N(x_n|\bm{0},\bm{I}_q)}}} \\
		=&-\frac{Nq}{2}\ln{2\pi}-\frac{1}{2}\sum_{n=1}^{N}{\Eq{\|x_n\|^2}} \\
		=&-\frac{1}{2}\sum_{n=1}^{N}{\Eq{\|x_n\|^2}} + const
	\end{align}	
		
	\begin{align}
		\Eq{\ln{p(\bm{m})}}=&\Eq{\ln{N(\bm{m}|\bm{0},\beta^{-1}\bm{I}_d)}}\\
		=&\Eq{-\frac{d}{2}\ln{2\pi}-\frac{1}{2}\ln{\Det{\beta^{-1}\bm{I}_d}}-\frac{1}{2}\bm{m}^T\beta I_d\bm{\mu}} \\
		=&-\frac{\beta}{2}\Eq{\|\bm{m}\|^2}+const \\
	\end{align}	
	
	\begin{align}
		\Eq{\ln{p(\bm{W} \vert z)}}=&\Eq{\ln{\prod_{i=1}^d\prod_{j=1}^q{\frac{1}{\sqrt{2\pi z_{i,j}}}\exp\left(-\frac{w_{i,j}^2}{2z_{i,j}} \right)}}} \\
		=&-\frac{1}{2}\sum_{i=1}^d\sum_{j=1}^q{\Eq{\ln{z_{i,j}}}+\frac{\Eq{w_{i,j}^2}}{\Eq{z_{i,j}}}} + const \\
		=&-\frac{1}{2}\sum_{i=1}^d\sum_{j=1}^q{\Eq{\ln{z_{i,j}}}+\frac{\Eq{w_{i,j}^2}}{\Eq{z_{i,j}}}} + const
	\end{align}		
	
	\begin{align}
		\Eq{\ln{p(z)}}=&\Eq{\ln{\prod_{i=1}^d\prod_{j=1}^q{\frac{1}{z_{i,j}}}}} \\
		=&-\sum_{i=1}^d\sum_{j=1}^q{\Eq{\ln{z_{i,j}}}}
	\end{align}		
	
	\begin{align}
		\Eq{\ln{p(\sigma^{-2})}}=&\Eq{\ln{\Gamma(\sigma^{-2} \vert c,d)}}\\
		=&\psi(\tilde{c}_{\sigma^{-2}})-\ln(\tilde{d}_{\sigma^{-2}}) \\
		=&-\ln(\tilde{d}_{\sigma^{-2}}) + const
	\end{align}

	
	\begin{align}
		\Eq{\ln{Q(\theta)}}=&\Eq{\ln{\prod_i{Q_i(\theta_i)}}} \\
		=&\Eq{\sum_i{\ln{Q_i(\theta_i)}}} \\
		=&\underbrace{\Eq{\ln{Q(\bm{X})}}}_{(9)} + \underbrace{\Eq{\ln{Q(\bm{m})}}}_{(10)} + \underbrace{\Eq{\ln{Q(\bm{W})}}}_{(11)} + \\
		&  \underbrace{\Eq{\ln{Q(z_{i,j})}}}_{(12)} + \underbrace{\Eq{\ln{Q(\sigma^{-2})}}}_{(13)} \nonumber
	\end{align}

	\begin{align}
		-\Eq{\ln{Q(\bm{X})}}&=-\Eq{\ln{\prod_{n=1}^N{\N[\bm{x}_n \vert \mu_x]{\Sigma_x}}}} \\
		&=\sum_{n=1}^N{-\Eq{\ln{\N[\bm{x}_n \vert \mu_x]{\Sigma_x}}}} \\
		&=\sum_{n=1}^N{\frac{q}{2}(1+\ln(2\pi)) + \frac{1}{2}\ln{\Det{\Sigma_x}}} \\
		&=\frac{Nq}{2}( 1+\ln(2\pi)) + \frac{N}{2}\ln{\Det{\Sigma_x}} \\
		&=\frac{N}{2}\ln{\Det{\Sigma_x}} + const
	\end{align}
	
	\begin{align}
		-\Eq{\ln{Q(\bm{m})}}&=-\Eq{\ln{\N[\mu_m]{\Sigma_m}}} \\
		&=\frac{q}{2}( 1+\ln(2\pi)) + \frac{1}{2}\ln{\Det{\Sigma_m}} \\
		&=\frac{1}{2}\ln{\Det{\Sigma_m}} + const
	\end{align}

	\begin{align}
		-\Eq{\ln{Q(\bm{W})}}&=-\Eq{\ln{\prod_{i=1}^d{\N[\bm{W}_i \vert \mu_{\bm{W}_i}]{\Sigma_{\bm{W}_i}}}}} \\
		&=\sum_{i=1}^d{-\Eq{\ln{\N[{\bm{W}_i} \vert \mu_{\bm{W}_i}]{\Sigma_{\bm{W}_i}}}}} \\
		&=\frac{dq}{2}(1+\ln(2\pi)) + \sum_{i=1}^d{\frac{1}{2}\ln{\Det{\Sigma_{\bm{W}_i}}}} \\
		&=\frac{1}{2}\sum_{i=1}^d{\ln{\Det{\Sigma_{\bm{W}_i}}}} + const
	\end{align}
	
	\begin{align}
		-\Eq{\ln{Q(\sigma^{-2})}}=&-\Eq{\ln{\Gamma(\sigma^{-2} \vert c,d)}} \\
		=&c-\ln{d}+\ln{\Gamma(c)}+(1-c)\psi(c) \\
		=&-\ln{d} + const
	\end{align}
	
	\begin{align}
		\ln{Q^*(z_{i,j})} \propto &\mathbb{E}_{\bm{X},\bm{W},\bm{m},\sigma^{-2}}\left[\ln{p(\bm{t},\bm{X},\bm{m},\bm{W},z,\sigma^{-2})} \right] \\
		=&\mathbb{E}_{W} \left[ \ln{p(W \vert z)} \right] + \ln{p(z_{i,j})} + const \\
		=&\mathbb{E}_{W} \left[ -\frac{1}{2}\ln{2\pi z_{i,j}} - \frac{w_{i,j}^2}{2z_{i,j}} \right] + \ln{\frac{1}{z_{i,j}}} + const \\
		=& -\frac{ \mathbb{E}_{W} \left[ w_{i,j}^2 \right] }{2z_{i,j}} -\frac{1}{2}\ln{2\pi z_{i,j}} + \ln{\frac{1}{z_{i,j}}} + const \\
	\end{align}	
	
	\begin{align}
		Q(z_{i,j})=&\frac{\exp(\ln{Q^*(z_{i,j}))}}{\int{\exp(\ln{Q^*(z_{i,j}))}} \, dz_{i,j}} + const \\
		=&\frac{\frac{1}{z_{i,j}\sqrt{2\pi z_{i,j}}}\exp \left( -\frac{ \mathbb{E}_{W} \left[ w_{i,j}^2 \right] }{2z_{i,j}} \right)}{\int{\frac{1}{z_{i,j}\sqrt{2\pi z_{i,j}}}\exp \left( -\frac{ \mathbb{E}_{W} \left[ w_{i,j}^2 \right] }{2z_{i,j}} \right) \, dz_{i,j}}} + const \\
		=&\frac{\frac{\left( \mathbb{E}_{W} \left[ w_{i,j}^2 \right]/2 \right)^{1/2}}{\sqrt{\pi}} z_{i,j}^{-1/2-1}\exp \left( -\frac{\mathbb{E}_{W} \left[ w_{i,j}^2 \right]/2}{z_{i,j}} \right)}{\int{\frac{\left( \mathbb{E}_{W} \left[ w_{i,j}^2 \right]/2 \right)^{1/2}}{\sqrt{\pi}} z_{i,j}^{-1/2-1}\exp \left( -\frac{\mathbb{E}_{W} \left[ w_{i,j}^2 \right]/2}{z_{i,j}} \right) \, dz_{i,j}}} + const \\
		=&\frac{\text{Inv-Gamma}(z_{i,j}|1/2,\mathbb{E}_{W} \left[ w_{i,j}^2 \right]/2)}{\int \text{Inv-Gamma}(z_{i,j}|1/2,\mathbb{E}_{W} \left[ w_{i,j}^2 \right]/2)dz_{i,j}} \\
		=&\text{Inv-Gamma}(z_{i,j}|1/2,\mathbb{E}_{W} \left[ w_{i,j}^2 \right]/2)
	\end{align}
	
	\begin{align}
		-\Eq{\ln{Q(z_{i,j})}}=&-\Eq{\text{Inv-Gamma}(z_{i,j}|1/2,\Eq{w_{i,j}^2}/2)} \\
		=&1/2+\ln{\frac{\Eq{w_{i,j}^2}}{2}\sqrt{\pi}}-(1+1/2)\psi(1/2) \\
		=&\ln{\Eq{w_{i,j}^2}} + const
	\end{align}
	
\end{document}
